matching-logic/src/Theories/FOEquality_ProofSystem.v
@@ -204,7 +204,7 @@ Proof.
   pose proof (bott_not_defined Γ) as H.
   use AnyReasoning in H.
   mlApplyMeta H.
-  fromMLGoal. wf_auto2.
+  fromMLGoal.
 
   apply ceil_monotonic; auto.
   { wf_auto2. }
